<?xml version="1.0"?>
<rdf:RDF xmlns="https://www.usc.gal/pcc/app/emofinder/"
     xml:base="https://www.usc.gal/pcc/app/emofinder/"
     xmlns:dc="http://purl.org/dc/elements/1.1/"
     xmlns:ns="http://creativecommons.org/ns#"
     xmlns:mod="https://w3id.org/mod#"
     xmlns:ns1="http://www.w3.org/2003/06/sw-vocab-status/ns#"
     xmlns:owl="http://www.w3.org/2002/07/owl#"
     xmlns:rdf="http://www.w3.org/1999/02/22-rdf-syntax-ns#"
     xmlns:xml="http://www.w3.org/XML/1998/namespace"
     xmlns:xsd="http://www.w3.org/2001/XMLSchema#"
     xmlns:rdfs="http://www.w3.org/2000/01/rdf-schema#"
     xmlns:skos="http://www.w3.org/2004/02/skos/core#"
     xmlns:vann="http://purl.org/vocab/vann/"
     xmlns:terms="http://purl.org/dc/terms/"
     xmlns:emofind="https://www.usc.gal/pcc/app/emofinder/"
     xmlns:emoskos="https://www.usc.gal/pcc/app/emofinder/kos/">
    <owl:Ontology rdf:about="https://www.usc.gal/pcc/app/emofinder/">
        <owl:imports rdf:resource="http://www.w3.org/2004/02/skos/core"/>
        <dc:creator>David Chaves Fraga</dc:creator>
        <dc:creator>Patricia Martín Chozas</dc:creator>
        <dc:creator>Óscar Hidlago Gerpe</dc:creator>
        <dc:title>Ontology for emotional words - Semantic Emofinder</dc:title>
        <owl:versionInfo>1.0</owl:versionInfo>
        <mod:createdWith rdf:resource="https://chowlk.linkeddata.es/"/>
    </owl:Ontology>
    


    <!-- 
    ///////////////////////////////////////////////////////////////////////////////////////
    //
    // Annotation properties
    //
    ///////////////////////////////////////////////////////////////////////////////////////
     -->

    


    <!-- http://purl.org/dc/elements/1.1/creator -->

    <owl:AnnotationProperty rdf:about="http://purl.org/dc/elements/1.1/creator"/>
    


    <!-- http://purl.org/dc/elements/1.1/source -->

    <owl:AnnotationProperty rdf:about="http://purl.org/dc/elements/1.1/source">
        <skos:scopeNote xml:lang="en">A related resource from which the described resource is derived.</skos:scopeNote>
    </owl:AnnotationProperty>
    


    <!-- http://purl.org/dc/elements/1.1/title -->

    <owl:AnnotationProperty rdf:about="http://purl.org/dc/elements/1.1/title"/>
    


    <!-- http://www.w3.org/2002/07/owl#versionInfo -->

    <owl:AnnotationProperty rdf:about="http://www.w3.org/2002/07/owl#versionInfo"/>
    


    <!-- http://www.w3.org/2003/06/sw-vocab-status/ns#term_status -->

    <owl:AnnotationProperty rdf:about="http://www.w3.org/2003/06/sw-vocab-status/ns#term_status"/>
    


    <!-- http://www.w3.org/2004/02/skos/core#scopeNote -->

    <owl:AnnotationProperty rdf:about="http://www.w3.org/2004/02/skos/core#scopeNote"/>
    


    <!-- https://w3id.org/mod#createdWith -->

    <owl:AnnotationProperty rdf:about="https://w3id.org/mod#createdWith"/>
    


    <!-- 
    ///////////////////////////////////////////////////////////////////////////////////////
    //
    // Object Properties
    //
    ///////////////////////////////////////////////////////////////////////////////////////
     -->

    


    <!-- http://purl.org/dc/terms/rights -->

    <owl:ObjectProperty rdf:about="http://purl.org/dc/terms/rights">
        <skos:scopeNote xml:lang="en">Used to describe rights related to a bibliographic resource.</skos:scopeNote>
    </owl:ObjectProperty>
    


    <!-- http://www.w3.org/ns/lemon/lime#entry -->

    <owl:ObjectProperty rdf:about="http://www.w3.org/ns/lemon/lime#entry">
        <rdfs:domain rdf:resource="http://www.w3.org/ns/lemon/lime#Lexicon"/>
        <rdfs:range rdf:resource="http://www.w3.org/ns/lemon/ontolex#LexicalEntry"/>
        <rdfs:comment xml:lang="en">The &apos;entry&apos; property relates a lexicon to one of the lexical entries contained in it.</rdfs:comment>
        <rdfs:comment xml:lang="ru">Свойство &apos;запись&apos; связывает лексикон с одной из содержащихся в нем словарных единиц.</rdfs:comment>
        <rdfs:isDefinedBy>http://www.w3.org/ns/lemon/lime</rdfs:isDefinedBy>
        <rdfs:label xml:lang="de">Eintrag</rdfs:label>
        <rdfs:label xml:lang="nl">Item</rdfs:label>
        <rdfs:label xml:lang="es">entrada</rdfs:label>
        <rdfs:label xml:lang="pt">entrada</rdfs:label>
        <rdfs:label xml:lang="it">entrata</rdfs:label>
        <rdfs:label xml:lang="en">entry</rdfs:label>
        <rdfs:label xml:lang="fr">entrée</rdfs:label>
        <rdfs:label xml:lang="sv">ingång</rdfs:label>
        <rdfs:label xml:lang="af">inskrywing</rdfs:label>
        <rdfs:label xml:lang="ro">înregistrare</rdfs:label>
        <rdfs:label xml:lang="ru">запись</rdfs:label>
        <ns1:term_status>stable</ns1:term_status>
    </owl:ObjectProperty>
    


    <!-- http://www.w3.org/ns/lemon/ontolex#canonicalForm -->

    <owl:ObjectProperty rdf:about="http://www.w3.org/ns/lemon/ontolex#canonicalForm"/>
    


    <!-- http://www.w3.org/ns/lemon/ontolex#lexicalForm -->

    <owl:ObjectProperty rdf:about="http://www.w3.org/ns/lemon/ontolex#lexicalForm"/>
    


    <!-- https://www.usc.gal/pcc/app/emofinder/affects -->

    <owl:ObjectProperty rdf:about="https://www.usc.gal/pcc/app/emofinder/affects">
        <rdfs:domain rdf:resource="https://www.usc.gal/pcc/app/emofinder/Annotation"/>
        <rdfs:comment xml:lang="en">Esta propiedad asigna una Anotación a una Lexical Entry.</rdfs:comment>
        <rdfs:label xml:lang="es">affecta a</rdfs:label>
        <rdfs:label xml:lang="en">affects</rdfs:label>
    </owl:ObjectProperty>
    


    <!-- https://www.usc.gal/pcc/app/emofinder/value -->

    <owl:ObjectProperty rdf:about="https://www.usc.gal/pcc/app/emofinder/value">
        <rdfs:domain>
            <owl:Restriction>
                <owl:onProperty rdf:resource="https://www.usc.gal/pcc/app/emofinder/value"/>
                <owl:allValuesFrom rdf:resource="https://www.usc.gal/pcc/app/emofinder/RecognitionTime"/>
            </owl:Restriction>
        </rdfs:domain>
        <rdfs:range rdf:resource="http://www.w3.org/2001/XMLSchema#Float"/>
    </owl:ObjectProperty>
    


    <!-- 
    ///////////////////////////////////////////////////////////////////////////////////////
    //
    // Data properties
    //
    ///////////////////////////////////////////////////////////////////////////////////////
     -->

    


    <!-- http://www.w3.org/ns/lemon/lime#language -->

    <owl:DatatypeProperty rdf:about="http://www.w3.org/ns/lemon/lime#language"/>
    


    <!-- https://w3id.org/riverbench/schema/metadata#mean -->

    <owl:DatatypeProperty rdf:about="https://w3id.org/riverbench/schema/metadata#mean">
        <rdfs:subPropertyOf rdf:resource="https://w3id.org/riverbench/schema/metadata#statisticalProperty"/>
        <rdfs:range rdf:resource="http://www.w3.org/2001/XMLSchema#double"/>
        <rdfs:comment xml:lang="en">Arithmetic mean of a distribution</rdfs:comment>
        <rdfs:label xml:lang="en">Mean</rdfs:label>
    </owl:DatatypeProperty>
    


    <!-- https://w3id.org/riverbench/schema/metadata#standardDeviation -->

    <owl:DatatypeProperty rdf:about="https://w3id.org/riverbench/schema/metadata#standardDeviation">
        <rdfs:subPropertyOf rdf:resource="https://w3id.org/riverbench/schema/metadata#statisticalProperty"/>
        <rdfs:range rdf:resource="http://www.w3.org/2001/XMLSchema#double"/>
        <rdfs:comment xml:lang="en">Standard deviation of a distribution</rdfs:comment>
        <rdfs:label xml:lang="en">Standard deviation</rdfs:label>
    </owl:DatatypeProperty>
    


    <!-- https://w3id.org/riverbench/schema/metadata#statisticalProperty -->

    <owl:DatatypeProperty rdf:about="https://w3id.org/riverbench/schema/metadata#statisticalProperty"/>
    


    <!-- https://www.usc.gal/pcc/app/emofinder/value -->

    <owl:DatatypeProperty rdf:about="https://www.usc.gal/pcc/app/emofinder/value"/>
    


    <!-- 
    ///////////////////////////////////////////////////////////////////////////////////////
    //
    // Classes
    //
    ///////////////////////////////////////////////////////////////////////////////////////
     -->

    


    <!-- http://purl.org/ontology/bibo/Article -->

    <owl:Class rdf:about="http://purl.org/ontology/bibo/Article">
        <rdfs:subClassOf rdf:resource="http://purl.org/ontology/bibo/Document"/>
        <rdfs:comment xml:lang="en">A written composition in prose, usually nonfiction, on a specific topic, forming an independent part of a book or other publication, as a newspaper or magazine.</rdfs:comment>
        <rdfs:isDefinedBy rdf:datatype="http://www.w3.org/2001/XMLSchema#anyURI">http://purl.org/ontology/bibo/</rdfs:isDefinedBy>
        <rdfs:label xml:lang="en">Article</rdfs:label>
        <ns1:term_status>stable</ns1:term_status>
    </owl:Class>
    


    <!-- http://purl.org/ontology/bibo/Document -->

    <owl:Class rdf:about="http://purl.org/ontology/bibo/Document"/>
    


    <!-- http://rdfs.org/ns/void#Dataset -->

    <owl:Class rdf:about="http://rdfs.org/ns/void#Dataset"/>
    


    <!-- http://www.ontologydesignpatterns.org/cp/owl/semiotics.owl#Expression -->

    <owl:Class rdf:about="http://www.ontologydesignpatterns.org/cp/owl/semiotics.owl#Expression"/>
    


    <!-- http://www.w3.org/2001/XMLSchema#Boolean -->

    <owl:Class rdf:about="http://www.w3.org/2001/XMLSchema#Boolean"/>
    


    <!-- http://www.w3.org/2001/XMLSchema#Float -->

    <owl:Class rdf:about="http://www.w3.org/2001/XMLSchema#Float"/>
    


    <!-- http://www.w3.org/2001/XMLSchema#String -->

    <owl:Class rdf:about="http://www.w3.org/2001/XMLSchema#String"/>
    


    <!-- http://www.w3.org/2004/02/skos/core#Concept -->

    <owl:Class rdf:about="http://www.w3.org/2004/02/skos/core#Concept">
        <rdfs:label>Concept</rdfs:label>
    </owl:Class>
    


    <!-- http://www.w3.org/ns/lemon/lime#Lexicon -->

    <owl:Class rdf:about="http://www.w3.org/ns/lemon/lime#Lexicon">
        <rdfs:subClassOf rdf:resource="http://rdfs.org/ns/void#Dataset"/>
        <rdfs:subClassOf>
            <owl:Restriction>
                <owl:onProperty rdf:resource="http://www.w3.org/ns/lemon/lime#entry"/>
                <owl:minQualifiedCardinality rdf:datatype="http://www.w3.org/2001/XMLSchema#nonNegativeInteger">1</owl:minQualifiedCardinality>
                <owl:onClass rdf:resource="http://www.w3.org/ns/lemon/ontolex#LexicalEntry"/>
            </owl:Restriction>
        </rdfs:subClassOf>
        <rdfs:subClassOf>
            <owl:Restriction>
                <owl:onProperty rdf:resource="http://www.w3.org/ns/lemon/lime#language"/>
                <owl:cardinality rdf:datatype="http://www.w3.org/2001/XMLSchema#nonNegativeInteger">1</owl:cardinality>
            </owl:Restriction>
        </rdfs:subClassOf>
        <rdfs:comment xml:lang="en">A lexicon represents a collection of lexical entries for a particular language or domain.</rdfs:comment>
        <rdfs:comment xml:lang="ru">Лексикон представляет собой набор словарных единиц для определенного языка или домена.</rdfs:comment>
        <rdfs:isDefinedBy>http://www.w3.org/ns/lemon/lime</rdfs:isDefinedBy>
        <rdfs:label xml:lang="it">Lessico</rdfs:label>
        <rdfs:label xml:lang="nl">Lexicon</rdfs:label>
        <rdfs:label xml:lang="de">Lexikon</rdfs:label>
        <rdfs:label xml:lang="fr">Lexique</rdfs:label>
        <rdfs:label xml:lang="af">leksikon</rdfs:label>
        <rdfs:label xml:lang="en">lexicon</rdfs:label>
        <rdfs:label xml:lang="ro">lexicon</rdfs:label>
        <rdfs:label xml:lang="es">lexicón</rdfs:label>
        <rdfs:label xml:lang="sv">lexikon</rdfs:label>
        <rdfs:label xml:lang="ru">лексикон</rdfs:label>
        <ns1:term_status>stable</ns1:term_status>
    </owl:Class>
    


    <!-- http://www.w3.org/ns/lemon/ontolex#Form -->

    <owl:Class rdf:about="http://www.w3.org/ns/lemon/ontolex#Form"/>
    


    <!-- http://www.w3.org/ns/lemon/ontolex#LexicalEntry -->

    <owl:Class rdf:about="http://www.w3.org/ns/lemon/ontolex#LexicalEntry">
        <rdfs:subClassOf rdf:resource="http://www.ontologydesignpatterns.org/cp/owl/semiotics.owl#Expression"/>
        <rdfs:subClassOf rdf:resource="http://www.w3.org/2002/07/owl#Thing"/>
        <rdfs:subClassOf>
            <owl:Restriction>
                <owl:onProperty rdf:resource="http://www.w3.org/ns/lemon/ontolex#lexicalForm"/>
                <owl:minQualifiedCardinality rdf:datatype="http://www.w3.org/2001/XMLSchema#nonNegativeInteger">1</owl:minQualifiedCardinality>
                <owl:onClass rdf:resource="http://www.w3.org/ns/lemon/ontolex#Form"/>
            </owl:Restriction>
        </rdfs:subClassOf>
        <rdfs:subClassOf>
            <owl:Restriction>
                <owl:onProperty rdf:resource="http://www.w3.org/ns/lemon/ontolex#canonicalForm"/>
                <owl:maxQualifiedCardinality rdf:datatype="http://www.w3.org/2001/XMLSchema#nonNegativeInteger">1</owl:maxQualifiedCardinality>
                <owl:onClass rdf:resource="http://www.w3.org/ns/lemon/ontolex#Form"/>
            </owl:Restriction>
        </rdfs:subClassOf>
        <rdfs:comment xml:lang="ru">&apos;Словарная единица&apos; представляет собой единицу анализа словаря, которая состоит из совокупности грамматически связанных форм и совокупности основных значений, ассоциирующихся со всеми этими формами. &apos;Словарная единица&apos; - это слово, словосочетание или аффикс одной части речи, морфологической модели, этимологии и набора значений.</rdfs:comment>
        <rdfs:comment xml:lang="en">A lexical entry represents a unit of analysis of the lexicon that consists of a set of forms that are grammatically related and a set of base meanings that are associated with all of these forms. Thus, a lexical entry is a word, multiword expression or affix with a single part-of-speech, morphological pattern, etymology and set of senses.</rdfs:comment>
        <rdfs:isDefinedBy rdf:resource="http://www.w3.org/ns/lemon/ontolex"/>
        <rdfs:label xml:lang="de">Lexikoneintrag</rdfs:label>
        <rdfs:label xml:lang="es">entrada léxica</rdfs:label>
        <rdfs:label xml:lang="it">entrata lessicale</rdfs:label>
        <rdfs:label xml:lang="fr">entrée lexicale</rdfs:label>
        <rdfs:label xml:lang="af">leksikale inskrywing</rdfs:label>
        <rdfs:label xml:lang="en">lexical entry</rdfs:label>
        <rdfs:label xml:lang="nl">lexikaal item</rdfs:label>
        <rdfs:label xml:lang="sv">lexikoningång</rdfs:label>
        <rdfs:label xml:lang="ro">înregistrare lexicală</rdfs:label>
        <rdfs:label xml:lang="ru">словарная единица</rdfs:label>
        <ns1:term_status>stable</ns1:term_status>
    </owl:Class>
    


    <!-- https://www.usc.gal/pcc/app/emofinder/AcquisitionAge -->

    <owl:Class rdf:about="https://www.usc.gal/pcc/app/emofinder/AcquisitionAge">
        <rdfs:subClassOf rdf:resource="https://www.usc.gal/pcc/app/emofinder/SubjectiveDimension"/>
        <rdfs:comment xml:lang="es">Esta variable indica la edad aproximada (en años) a la que un individuo cree que aprendió una determinada palabra.</rdfs:comment>
        <rdfs:comment xml:lang="en">This variable indicates the approximate age (in years) at which an individual believes they learned a particular word.</rdfs:comment>
        <rdfs:label xml:lang="en">Acquisition Age</rdfs:label>
        <rdfs:label xml:lang="es">Edad de adquisición</rdfs:label>
    </owl:Class>
    


    <!-- https://www.usc.gal/pcc/app/emofinder/Action -->

    <owl:Class rdf:about="https://www.usc.gal/pcc/app/emofinder/Action">
        <rdfs:subClassOf rdf:resource="https://www.usc.gal/pcc/app/emofinder/SubjectiveDimension"/>
        <rdfs:comment xml:lang="en">It refers to the degree of the word&apos;s connection with acting, doing, and influencing.</rdfs:comment>
        <rdfs:comment xml:lang="es">Se refiere al grado de relación de la palabra con actuar, hacer, e influir.</rdfs:comment>
        <rdfs:label xml:lang="en">Action</rdfs:label>
        <rdfs:label xml:lang="es">Actuación</rdfs:label>
    </owl:Class>
    


    <!-- https://www.usc.gal/pcc/app/emofinder/Amusement -->

    <owl:Class rdf:about="https://www.usc.gal/pcc/app/emofinder/Amusement">
        <rdfs:subClassOf rdf:resource="https://www.usc.gal/pcc/app/emofinder/DiscreteEmotionalCategory"/>
        <rdfs:comment xml:lang="en">It refers to the degree of amusement conveyed by a word.</rdfs:comment>
        <rdfs:comment xml:lang="es">Se refiere al grado de diversión que transmite una palabra.</rdfs:comment>
        <rdfs:label xml:lang="en">Amusement</rdfs:label>
        <rdfs:label xml:lang="es">Diversión</rdfs:label>
    </owl:Class>
    


    <!-- https://www.usc.gal/pcc/app/emofinder/Anger -->

    <owl:Class rdf:about="https://www.usc.gal/pcc/app/emofinder/Anger">
        <rdfs:subClassOf rdf:resource="https://www.usc.gal/pcc/app/emofinder/DiscreteEmotionalCategory"/>
        <rdfs:comment xml:lang="en">It refers to the degree of anger conveyed by a word.</rdfs:comment>
        <rdfs:comment xml:lang="es">Se refiere al grado de enfado que transmite una palabra.</rdfs:comment>
        <rdfs:label xml:lang="en">Anger</rdfs:label>
        <rdfs:label xml:lang="es">Enfado</rdfs:label>
    </owl:Class>
    


    <!-- https://www.usc.gal/pcc/app/emofinder/Annotation -->

    <owl:Class rdf:about="https://www.usc.gal/pcc/app/emofinder/Annotation">
        <rdfs:label xml:lang="en">Annotation</rdfs:label>
        <rdfs:label xml:lang="es">Anotación</rdfs:label>
    </owl:Class>
    


    <!-- https://www.usc.gal/pcc/app/emofinder/Arousal -->

    <owl:Class rdf:about="https://www.usc.gal/pcc/app/emofinder/Arousal">
        <rdfs:subClassOf rdf:resource="https://www.usc.gal/pcc/app/emofinder/EmotionalDimension"/>
        <rdfs:comment xml:lang="en">Arousal refers to the level of calmness or excitement evoked by a word, that is, how relaxing or intense it feels to the person.</rdfs:comment>
        <rdfs:comment xml:lang="es">La activación hace referencia al nivel de calma o excitación que evoca una palabra, es decir, cuán relajante o intensa le resulta a la persona.</rdfs:comment>
        <rdfs:label xml:lang="es">Activación</rdfs:label>
        <rdfs:label xml:lang="en">Arousal</rdfs:label>
    </owl:Class>
    


    <!-- https://www.usc.gal/pcc/app/emofinder/Awe -->

    <owl:Class rdf:about="https://www.usc.gal/pcc/app/emofinder/Awe">
        <rdfs:subClassOf rdf:resource="https://www.usc.gal/pcc/app/emofinder/DiscreteEmotionalCategory"/>
        <rdfs:comment xml:lang="en">It refers to the degree of awe conveyed by a word.</rdfs:comment>
        <rdfs:comment xml:lang="es">Se refiere al grado de admiración que transmite una palabra.</rdfs:comment>
        <rdfs:label xml:lang="es">Admiración</rdfs:label>
        <rdfs:label xml:lang="en">Awe</rdfs:label>
    </owl:Class>
    


    <!-- https://www.usc.gal/pcc/app/emofinder/BodyExpression -->

    <owl:Class rdf:about="https://www.usc.gal/pcc/app/emofinder/BodyExpression">
        <rdfs:subClassOf rdf:resource="https://www.usc.gal/pcc/app/emofinder/SubjectiveDimension"/>
        <rdfs:comment xml:lang="en">It refers to the degree of the word&apos;s connection with changes in parts of the body such as the voice, posture, gestures, or facial expression.</rdfs:comment>
        <rdfs:comment xml:lang="es">Se refiere al grado de relación de la palabra con cambios en partes del cuerpo como la voz, la postura, los gestos, o la expresión de la cara</rdfs:comment>
        <rdfs:label xml:lang="en">Body Expression</rdfs:label>
        <rdfs:label xml:lang="es">Expresión Corporal</rdfs:label>
    </owl:Class>
    


    <!-- https://www.usc.gal/pcc/app/emofinder/Concreteness -->

    <owl:Class rdf:about="https://www.usc.gal/pcc/app/emofinder/Concreteness">
        <rdfs:subClassOf rdf:resource="https://www.usc.gal/pcc/app/emofinder/SubjectiveDimension"/>
        <rdfs:comment xml:lang="en">Concreteness refers to the extent to which a word refers to an entity that can be perceived with the senses.</rdfs:comment>
        <rdfs:comment xml:lang="es">La concreción se refiere a hasta qué punto la palabra se refiere a una entidad que puede percibirse con los sentidos.</rdfs:comment>
        <rdfs:label xml:lang="es">Concreción</rdfs:label>
        <rdfs:label xml:lang="en">Concreteness</rdfs:label>
    </owl:Class>
    


    <!-- https://www.usc.gal/pcc/app/emofinder/Contentment -->

    <owl:Class rdf:about="https://www.usc.gal/pcc/app/emofinder/Contentment">
        <rdfs:subClassOf rdf:resource="https://www.usc.gal/pcc/app/emofinder/DiscreteEmotionalCategory"/>
        <rdfs:comment xml:lang="en">It refers to the degree of contentment conveyed by a word.</rdfs:comment>
        <rdfs:comment xml:lang="es">Se refiere al grado de satisfacción que transmite una palabra.</rdfs:comment>
        <rdfs:label xml:lang="en">Contentment</rdfs:label>
        <rdfs:label xml:lang="es">Satisfacción</rdfs:label>
    </owl:Class>
    


    <!-- https://www.usc.gal/pcc/app/emofinder/ContextualAvailability -->

    <owl:Class rdf:about="https://www.usc.gal/pcc/app/emofinder/ContextualAvailability">
        <rdfs:subClassOf rdf:resource="https://www.usc.gal/pcc/app/emofinder/SubjectiveDimension"/>
        <rdfs:comment xml:lang="en">Contextual availability refers to the ease with which we can think of a context to which the word could be associated.</rdfs:comment>
        <rdfs:comment xml:lang="es">La disponibilidad contextual se refiere a la facilidad con la que podemos pensar en un contexto al cual se podría asociar la palabra.</rdfs:comment>
        <rdfs:label xml:lang="en">Contextual Availability</rdfs:label>
        <rdfs:label xml:lang="es">Disponibilidad contextual</rdfs:label>
    </owl:Class>
    


    <!-- https://www.usc.gal/pcc/app/emofinder/DiscreteEmotionalCategory -->

    <owl:Class rdf:about="https://www.usc.gal/pcc/app/emofinder/DiscreteEmotionalCategory">
        <rdfs:subClassOf rdf:resource="https://www.usc.gal/pcc/app/emofinder/Annotation"/>
        <rdfs:label xml:lang="es">Categoría emocional discreta</rdfs:label>
        <rdfs:label xml:lang="en">Discrete emotional category</rdfs:label>
    </owl:Class>
    


    <!-- https://www.usc.gal/pcc/app/emofinder/Disgust -->

    <owl:Class rdf:about="https://www.usc.gal/pcc/app/emofinder/Disgust">
        <rdfs:subClassOf rdf:resource="https://www.usc.gal/pcc/app/emofinder/DiscreteEmotionalCategory"/>
        <rdfs:comment xml:lang="en">It refers to the degree of disgust conveyed by a word.</rdfs:comment>
        <rdfs:comment xml:lang="es">Se refiere al grado de asco que transmite una palabra.</rdfs:comment>
        <rdfs:label xml:lang="es">Asco</rdfs:label>
        <rdfs:label xml:lang="en">Disgust</rdfs:label>
    </owl:Class>
    


    <!-- https://www.usc.gal/pcc/app/emofinder/Dominance -->

    <owl:Class rdf:about="https://www.usc.gal/pcc/app/emofinder/Dominance">
        <rdfs:subClassOf rdf:resource="https://www.usc.gal/pcc/app/emofinder/EmotionalDimension"/>
        <rdfs:comment xml:lang="en">Dominance refers to the perception of control evoked by a word, that is, the extent to which a person feels weak/submissive or strong/dominant in relation to the concept the word represents.</rdfs:comment>
        <rdfs:comment xml:lang="es">La dominancia hace referencia a la percepción de control que evoca una palabra, es decir, hasta qué punto la persona se siente débil/sumisa o fuerte/dominante ante el concepto que designa la palabra.</rdfs:comment>
        <rdfs:label xml:lang="en">Dominance</rdfs:label>
        <rdfs:label xml:lang="es">Dominancia</rdfs:label>
    </owl:Class>
    


    <!-- https://www.usc.gal/pcc/app/emofinder/EmotionalDimension -->

    <owl:Class rdf:about="https://www.usc.gal/pcc/app/emofinder/EmotionalDimension">
        <rdfs:subClassOf rdf:resource="https://www.usc.gal/pcc/app/emofinder/Annotation"/>
        <rdfs:label xml:lang="es">Dimensión emocional</rdfs:label>
        <rdfs:label xml:lang="en">Emotional Dimension</rdfs:label>
    </owl:Class>
    


    <!-- https://www.usc.gal/pcc/app/emofinder/Evaluation -->

    <owl:Class rdf:about="https://www.usc.gal/pcc/app/emofinder/Evaluation">
        <rdfs:subClassOf rdf:resource="https://www.usc.gal/pcc/app/emofinder/EmotionalDimension"/>
        <rdfs:comment xml:lang="en">It refers to the degree of the word&apos;s connection with situations that are important for well-being and/or survival.</rdfs:comment>
        <rdfs:comment xml:lang="es">Se refiere al grado de relación de la palabra con situaciones importantes para el bienestar y/o supervivencia.</rdfs:comment>
        <rdfs:label xml:lang="es">Evaluación</rdfs:label>
        <rdfs:label xml:lang="en">Evaluation</rdfs:label>
    </owl:Class>
    


    <!-- https://www.usc.gal/pcc/app/emofinder/Excitement -->

    <owl:Class rdf:about="https://www.usc.gal/pcc/app/emofinder/Excitement">
        <rdfs:subClassOf rdf:resource="https://www.usc.gal/pcc/app/emofinder/DiscreteEmotionalCategory"/>
        <rdfs:comment xml:lang="en">It refers to the degree of excitement conveyed by a word.</rdfs:comment>
        <rdfs:comment xml:lang="es">Se refiere al grado de entusiasmo que transmite una palabra.</rdfs:comment>
        <rdfs:label xml:lang="es">Entusiasmo</rdfs:label>
        <rdfs:label xml:lang="en">Excitement</rdfs:label>
    </owl:Class>
    


    <!-- https://www.usc.gal/pcc/app/emofinder/Familiarity -->

    <owl:Class rdf:about="https://www.usc.gal/pcc/app/emofinder/Familiarity">
        <rdfs:subClassOf rdf:resource="https://www.usc.gal/pcc/app/emofinder/SubjectiveDimension"/>
        <rdfs:comment xml:lang="en">Familiarity refers to how familiar or known a word feels to a person.</rdfs:comment>
        <rdfs:comment xml:lang="es">La familiaridad hace referencia a cuán familiar o conocida resulta una palabra para la persona.</rdfs:comment>
        <rdfs:label xml:lang="es">Familiaridad</rdfs:label>
        <rdfs:label xml:lang="en">Familiarity</rdfs:label>
    </owl:Class>
    


    <!-- https://www.usc.gal/pcc/app/emofinder/Fear -->

    <owl:Class rdf:about="https://www.usc.gal/pcc/app/emofinder/Fear">
        <rdfs:subClassOf rdf:resource="https://www.usc.gal/pcc/app/emofinder/DiscreteEmotionalCategory"/>
        <rdfs:comment xml:lang="en">It refers to the degree of fear conveyed by a word.</rdfs:comment>
        <rdfs:comment xml:lang="es">Se refiere al grado de miedo que transmite una palabra.</rdfs:comment>
        <rdfs:label xml:lang="en">Fear</rdfs:label>
        <rdfs:label xml:lang="es">Miedo</rdfs:label>
    </owl:Class>
    


    <!-- https://www.usc.gal/pcc/app/emofinder/Feeling -->

    <owl:Class rdf:about="https://www.usc.gal/pcc/app/emofinder/Feeling">
        <rdfs:subClassOf rdf:resource="https://www.usc.gal/pcc/app/emofinder/EmotionalDimension"/>
        <rdfs:comment xml:lang="en">It refers to the degree of the word&apos;s connection with feelings.</rdfs:comment>
        <rdfs:comment xml:lang="es">Se refiere al grado de relación de la palabra con sentimientos.</rdfs:comment>
        <rdfs:label xml:lang="en">Feeling</rdfs:label>
        <rdfs:label xml:lang="es">Sentimiento</rdfs:label>
    </owl:Class>
    


    <!-- https://www.usc.gal/pcc/app/emofinder/Happiness -->

    <owl:Class rdf:about="https://www.usc.gal/pcc/app/emofinder/Happiness">
        <rdfs:subClassOf rdf:resource="https://www.usc.gal/pcc/app/emofinder/DiscreteEmotionalCategory"/>
        <rdfs:comment xml:lang="en">It refers to the degree of happiness conveyed by a word.</rdfs:comment>
        <rdfs:comment xml:lang="es">Se refiere al grado de felicidad que transmite una palabra.</rdfs:comment>
        <rdfs:label xml:lang="es">Felicidad</rdfs:label>
        <rdfs:label xml:lang="en">Happiness</rdfs:label>
    </owl:Class>
    


    <!-- https://www.usc.gal/pcc/app/emofinder/Iconicity -->

    <owl:Class rdf:about="https://www.usc.gal/pcc/app/emofinder/Iconicity">
        <rdfs:subClassOf rdf:resource="https://www.usc.gal/pcc/app/emofinder/SubjectiveDimension"/>
        <rdfs:comment xml:lang="en">It refers to the degree of the word’s sound relation to its meaning.</rdfs:comment>
        <rdfs:comment xml:lang="es">Se refiere al grado de relación del sonido de la palabra con su significado.</rdfs:comment>
        <rdfs:label xml:lang="es">Iconicidad</rdfs:label>
        <rdfs:label xml:lang="en">Iconicity</rdfs:label>
    </owl:Class>
    


    <!-- https://www.usc.gal/pcc/app/emofinder/Imageability -->

    <owl:Class rdf:about="https://www.usc.gal/pcc/app/emofinder/Imageability">
        <rdfs:subClassOf rdf:resource="https://www.usc.gal/pcc/app/emofinder/SubjectiveDimension"/>
        <rdfs:comment xml:lang="en">Imaginability refers to the ease with which a mental image of the concept designated by the word can be formed.</rdfs:comment>
        <rdfs:comment xml:lang="es">La imaginabilidad hace referencia a la facilidad para formarse una imagen mental del concepto que designa la palabra.</rdfs:comment>
        <rdfs:label xml:lang="en">Imageability</rdfs:label>
        <rdfs:label xml:lang="es">Imaginabilidad</rdfs:label>
    </owl:Class>
    


    <!-- https://www.usc.gal/pcc/app/emofinder/Interoception -->

    <owl:Class rdf:about="https://www.usc.gal/pcc/app/emofinder/Interoception">
        <rdfs:subClassOf rdf:resource="https://www.usc.gal/pcc/app/emofinder/EmotionalDimension"/>
        <rdfs:comment xml:lang="en">It refers to the degree of the word&apos;s connection with internal bodily sensations.</rdfs:comment>
        <rdfs:comment xml:lang="es">Se refiere al grado de relación de la palabra con sensaciones corporales internas.</rdfs:comment>
        <rdfs:label xml:lang="es">Interocepción</rdfs:label>
        <rdfs:label xml:lang="en">Interoception</rdfs:label>
    </owl:Class>
    


    <!-- https://www.usc.gal/pcc/app/emofinder/Morality -->

    <owl:Class rdf:about="https://www.usc.gal/pcc/app/emofinder/Morality">
        <rdfs:subClassOf rdf:resource="https://www.usc.gal/pcc/app/emofinder/SubjectiveDimension"/>
        <rdfs:comment xml:lang="en">It refers to the degree of the word&apos;s connection with morality, rules, or any other principle that guides behavior.</rdfs:comment>
        <rdfs:comment xml:lang="es">Se refiere al grado de relación de la palabra con la moralidad, las reglas, o cualquier otro principio que guía la conducta.</rdfs:comment>
        <rdfs:label xml:lang="es">Moralidad</rdfs:label>
        <rdfs:label xml:lang="en">Morality</rdfs:label>
    </owl:Class>
    


    <!-- https://www.usc.gal/pcc/app/emofinder/ObjectiveAcquisitionAge -->

    <owl:Class rdf:about="https://www.usc.gal/pcc/app/emofinder/ObjectiveAcquisitionAge">
        <rdfs:subClassOf rdf:resource="https://www.usc.gal/pcc/app/emofinder/ObjectiveEstimation"/>
        <rdfs:comment xml:lang="en">It refers to the age at which the word was acquired.</rdfs:comment>
        <rdfs:comment xml:lang="es">Se refiere a la edad en la que se ha adquirido la palabra.</rdfs:comment>
        <rdfs:label xml:lang="es">Edad de adquisición objetiva</rdfs:label>
        <rdfs:label xml:lang="en">Objective Acquisition Age</rdfs:label>
    </owl:Class>
    


    <!-- https://www.usc.gal/pcc/app/emofinder/ObjectiveEstimation -->

    <owl:Class rdf:about="https://www.usc.gal/pcc/app/emofinder/ObjectiveEstimation">
        <rdfs:subClassOf rdf:resource="https://www.usc.gal/pcc/app/emofinder/Annotation"/>
        <rdfs:label xml:lang="es">Estimación Objetiva</rdfs:label>
        <rdfs:label xml:lang="en">Objective Estimation</rdfs:label>
    </owl:Class>
    


    <!-- https://www.usc.gal/pcc/app/emofinder/Pleasure -->

    <owl:Class rdf:about="https://www.usc.gal/pcc/app/emofinder/Pleasure">
        <rdfs:subClassOf rdf:resource="https://www.usc.gal/pcc/app/emofinder/DiscreteEmotionalCategory"/>
        <rdfs:comment xml:lang="en">It refers to the degree of pleasure conveyed by a word.</rdfs:comment>
        <rdfs:comment xml:lang="es">Se refiere al grado de placer que transmite una palabra.</rdfs:comment>
        <rdfs:label xml:lang="es">Placer</rdfs:label>
        <rdfs:label xml:lang="en">Pleasure</rdfs:label>
    </owl:Class>
    


    <!-- https://www.usc.gal/pcc/app/emofinder/Prototipicality -->

    <owl:Class rdf:about="https://www.usc.gal/pcc/app/emofinder/Prototipicality">
        <rdfs:subClassOf rdf:resource="https://www.usc.gal/pcc/app/emofinder/EmotionalDimension"/>
        <rdfs:comment xml:lang="en">It refers to the degree of the word’s connection with an emotion.</rdfs:comment>
        <rdfs:comment xml:lang="es">Se refiere al grado de relación de la palabra con una emoción.</rdfs:comment>
        <rdfs:label xml:lang="es">Prototipicalidad</rdfs:label>
        <rdfs:label xml:lang="en">Prototipicality</rdfs:label>
    </owl:Class>
    


    <!-- https://www.usc.gal/pcc/app/emofinder/RecognitionErrorPercentage -->

    <owl:Class rdf:about="https://www.usc.gal/pcc/app/emofinder/RecognitionErrorPercentage">
        <rdfs:subClassOf rdf:resource="https://www.usc.gal/pcc/app/emofinder/RecognitionTime"/>
        <rdfs:comment xml:lang="en">%E</rdfs:comment>
        <rdfs:comment xml:lang="en">Percentage of incorrect word identification in a lexical decision task.</rdfs:comment>
        <rdfs:comment xml:lang="es">Porcentaje de identificación incorrecta de la palabra en una tarea de decisión léxica.</rdfs:comment>
        <rdfs:label xml:lang="es">Porcentaje de error de reconocimiento (LDT)</rdfs:label>
        <rdfs:label xml:lang="en">Recognition Error Percentage</rdfs:label>
    </owl:Class>
    


    <!-- https://www.usc.gal/pcc/app/emofinder/RecognitionTime -->

    <owl:Class rdf:about="https://www.usc.gal/pcc/app/emofinder/RecognitionTime">
        <rdfs:subClassOf rdf:resource="https://www.usc.gal/pcc/app/emofinder/Annotation"/>
        <rdfs:label xml:lang="en">Recognition Time</rdfs:label>
        <rdfs:label xml:lang="es">Tiempo de reconocimiento</rdfs:label>
    </owl:Class>
    


    <!-- https://www.usc.gal/pcc/app/emofinder/Relief -->

    <owl:Class rdf:about="https://www.usc.gal/pcc/app/emofinder/Relief">
        <rdfs:subClassOf rdf:resource="https://www.usc.gal/pcc/app/emofinder/DiscreteEmotionalCategory"/>
        <rdfs:comment xml:lang="es">It refers to the degree of relief conveyed by a word.</rdfs:comment>
        <rdfs:comment xml:lang="es">Se refiere al grado de alivio que transmite una palabra.</rdfs:comment>
        <rdfs:label xml:lang="es">Alivio</rdfs:label>
        <rdfs:label xml:lang="en">Relief</rdfs:label>
    </owl:Class>
    


    <!-- https://www.usc.gal/pcc/app/emofinder/Sadness -->

    <owl:Class rdf:about="https://www.usc.gal/pcc/app/emofinder/Sadness">
        <rdfs:subClassOf rdf:resource="https://www.usc.gal/pcc/app/emofinder/DiscreteEmotionalCategory"/>
        <rdfs:comment xml:lang="en">It refers to the degree of sadness conveyed by a word.</rdfs:comment>
        <rdfs:comment xml:lang="es">Se refiere al grado de tristeza que transmite una palabra.</rdfs:comment>
        <rdfs:label xml:lang="en">Sadness</rdfs:label>
        <rdfs:label xml:lang="es">Tristeza</rdfs:label>
    </owl:Class>
    


    <!-- https://www.usc.gal/pcc/app/emofinder/SensoryExperience -->

    <owl:Class rdf:about="https://www.usc.gal/pcc/app/emofinder/SensoryExperience">
        <rdfs:subClassOf rdf:resource="https://www.usc.gal/pcc/app/emofinder/SubjectiveDimension"/>
        <rdfs:comment xml:lang="es">Indica hasta qué punto la palabra evoca una experiencia sensorial/perceptiva (sabor, tacto, vista, sonido y olor).</rdfs:comment>
        <rdfs:comment xml:lang="en">It indicates the extent to which the word evokes a sensory/perceptual experience (taste, touch, sight, sound, and smell).</rdfs:comment>
        <rdfs:label xml:lang="es">Experiencia sensorial</rdfs:label>
        <rdfs:label xml:lang="en">Sensory Experience</rdfs:label>
    </owl:Class>
    


    <!-- https://www.usc.gal/pcc/app/emofinder/Serenity -->

    <owl:Class rdf:about="https://www.usc.gal/pcc/app/emofinder/Serenity">
        <rdfs:subClassOf rdf:resource="https://www.usc.gal/pcc/app/emofinder/DiscreteEmotionalCategory"/>
        <rdfs:comment xml:lang="en">It refers to the degree of serenity conveyed by a word.</rdfs:comment>
        <rdfs:comment xml:lang="es">Se refiere al grado de serenidad que transmite una palabra.</rdfs:comment>
        <rdfs:label xml:lang="es">Serenidad</rdfs:label>
        <rdfs:label xml:lang="en">Serenity</rdfs:label>
    </owl:Class>
    


    <!-- https://www.usc.gal/pcc/app/emofinder/SocialInteraction -->

    <owl:Class rdf:about="https://www.usc.gal/pcc/app/emofinder/SocialInteraction">
        <rdfs:subClassOf rdf:resource="https://www.usc.gal/pcc/app/emofinder/SubjectiveDimension"/>
        <rdfs:label xml:lang="es">Interacción social</rdfs:label>
        <rdfs:label xml:lang="en">Social Interaction</rdfs:label>
    </owl:Class>
    


    <!-- https://www.usc.gal/pcc/app/emofinder/SubjectiveDimension -->

    <owl:Class rdf:about="https://www.usc.gal/pcc/app/emofinder/SubjectiveDimension">
        <rdfs:subClassOf rdf:resource="https://www.usc.gal/pcc/app/emofinder/Annotation"/>
        <rdfs:label xml:lang="es">Dimensión subjetiva</rdfs:label>
        <rdfs:label xml:lang="en">Subjective Dimension</rdfs:label>
    </owl:Class>
    


    <!-- https://www.usc.gal/pcc/app/emofinder/Thought -->

    <owl:Class rdf:about="https://www.usc.gal/pcc/app/emofinder/Thought">
        <rdfs:subClassOf rdf:resource="https://www.usc.gal/pcc/app/emofinder/SubjectiveDimension"/>
        <rdfs:comment xml:lang="en">It refers to the degree of the word&apos;s connection with mental activity, ideas, opinions, and judgments.</rdfs:comment>
        <rdfs:comment xml:lang="es">Se refiere al grado de relación de la palabra con la actividad mental, las ideas, las opiniones y los juicios.</rdfs:comment>
        <rdfs:label xml:lang="es">Pensamiento</rdfs:label>
        <rdfs:label xml:lang="en">Thought</rdfs:label>
    </owl:Class>
    


    <!-- https://www.usc.gal/pcc/app/emofinder/TimeNaming -->

    <owl:Class rdf:about="https://www.usc.gal/pcc/app/emofinder/TimeNaming">
        <rdfs:subClassOf rdf:resource="https://www.usc.gal/pcc/app/emofinder/RecognitionTime"/>
        <rdfs:comment xml:lang="en">Se refiere al tiempo de nombrado de la palabra, esto es, de lectura de la palabra en voz alta.</rdfs:comment>
        <rdfs:comment xml:lang="es">Se refiere al tiempo de nombrado de la palabra, esto es, de lectura de la palabra en voz alta.</rdfs:comment>
        <rdfs:label xml:lang="en">Naming time</rdfs:label>
        <rdfs:label xml:lang="es">Tiempo de nombrado</rdfs:label>
    </owl:Class>
    


    <!-- https://www.usc.gal/pcc/app/emofinder/TimeTdl -->

    <owl:Class rdf:about="https://www.usc.gal/pcc/app/emofinder/TimeTdl">
        <rdfs:subClassOf rdf:resource="https://www.usc.gal/pcc/app/emofinder/RecognitionTime"/>
        <rdfs:comment xml:lang="es">La variable tiempo de respuesta en tareas de Decisión Léxica se refiere al tiempo que tarda un participante en reconocer si un estímulo presentado es una palabra real, esto es, que existe en el idioma.</rdfs:comment>
        <rdfs:comment xml:lang="en">The variable response time in Lexical Decision tasks refers to the time it takes for a participant to recognize whether a presented stimulus is a real word, that is, one that exists in the language.</rdfs:comment>
        <rdfs:label xml:lang="en">Response time (TDL)</rdfs:label>
        <rdfs:label xml:lang="es">Tiempo de respuesta (LDT)</rdfs:label>
    </owl:Class>
    


    <!-- https://www.usc.gal/pcc/app/emofinder/Valence -->

    <owl:Class rdf:about="https://www.usc.gal/pcc/app/emofinder/Valence">
        <rdfs:subClassOf rdf:resource="https://www.usc.gal/pcc/app/emofinder/EmotionalDimension"/>
        <rdfs:comment xml:lang="es">La valencia hace referencia al nivel de agrado o desagrado que evoca una palabra, es decir, cuán positiva o negativa le resulta a la persona.</rdfs:comment>
        <rdfs:comment xml:lang="en">Valence refers to the level of pleasantness or unpleasantness evoked by a word, that is, how positive or negative it feels to the person.</rdfs:comment>
        <rdfs:label xml:lang="en">Valence</rdfs:label>
        <rdfs:label xml:lang="es">Valencia</rdfs:label>
    </owl:Class>
    


    <!-- 
    ///////////////////////////////////////////////////////////////////////////////////////
    //
    // Individuals
    //
    ///////////////////////////////////////////////////////////////////////////////////////
     -->

    


    <!-- https://www.usc.gal/pcc/app/emofinder/kos/Category -->

    <owl:NamedIndividual rdf:about="https://www.usc.gal/pcc/app/emofinder/kos/Category"/>
    


    <!-- 
    ///////////////////////////////////////////////////////////////////////////////////////
    //
    // Annotations
    //
    ///////////////////////////////////////////////////////////////////////////////////////
     -->

    <rdf:Description rdf:about="https://www.usc.gal/pcc/app/emofinder/value">
        <rdfs:label xml:lang="en">recognitionTime</rdfs:label>
    </rdf:Description>
</rdf:RDF>



<!-- Generated by the OWL API (version 4.5.9.2019-02-01T07:24:44Z) https://github.com/owlcs/owlapi -->

